07TreeCode/TreeCode.thy
@@ -26,7 +26,6 @@ datatype code\<^sub>e =
   | PushLam\<^sub>e "code\<^sub>e list" nat
   | Apply\<^sub>e
   | PushEnv\<^sub>e
-  | PopEnv\<^sub>e
   | Return\<^sub>e
   | Jump\<^sub>e
 
@@ -36,12 +35,6 @@ fun properly_terminated\<^sub>e :: "code\<^sub>e list \<Rightarrow> bool" where
 | "properly_terminated\<^sub>e (Return\<^sub>e # \<C>) = (\<C> = [])"
 | "properly_terminated\<^sub>e (Jump\<^sub>e # \<C>) = (\<C> = [])"
 | "properly_terminated\<^sub>e (op # \<C>) = properly_terminated\<^sub>e \<C>"
-
-fun pop_free :: "code\<^sub>e list \<Rightarrow> bool" where
-  "pop_free [] = True"
-| "pop_free (PushLam\<^sub>e \<C>' n # \<C>) = (pop_free \<C>' \<and> pop_free \<C>)"
-| "pop_free (PopEnv\<^sub>e # \<C>) = False"
-| "pop_free (op # \<C>) = pop_free \<C>"
 
 text \<open>Our closure-values remain the same, with just a change from a function body to a function 
 codeblock in closures-proper.\<close>
@@ -75,7 +68,6 @@ inductive eval\<^sub>e :: "state\<^sub>e \<Rightarrow> state\<^sub>e \<Rightarro
 | ev\<^sub>e_apply [simp]: "S\<^sub>e (v # Lam\<^sub>e \<Delta>' \<C>' n # \<V>) ((\<Delta>, Apply\<^sub>e # \<C>) # s) \<leadsto>\<^sub>e 
     S\<^sub>e \<V> (([v] # \<Delta>', \<C>') # (\<Delta>, \<C>) # s)"
 | ev\<^sub>e_pushenv [simp]: "S\<^sub>e (v # \<V>) ((\<Delta>, PushEnv\<^sub>e # \<C>) # s) \<leadsto>\<^sub>e S\<^sub>e \<V> ((cons_fst v \<Delta>, \<C>) # s)"
-| ev\<^sub>e_popenv [simp]: "S\<^sub>e \<V> (((v # vs) # \<Delta>, PopEnv\<^sub>e # \<C>) # s) \<leadsto>\<^sub>e S\<^sub>e \<V> ((vs # \<Delta>, \<C>) # s)"
 | ev\<^sub>e_return [simp]: "S\<^sub>e \<V> ((\<Delta>, Return\<^sub>e # \<C>) # s) \<leadsto>\<^sub>e S\<^sub>e \<V> s"
 | ev\<^sub>e_jump [simp]: "S\<^sub>e (v # Lam\<^sub>e \<Delta>' \<C>' n # \<V>) ((\<Delta>, Jump\<^sub>e # \<C>) # s) \<leadsto>\<^sub>e S\<^sub>e \<V> (([v] # \<Delta>', \<C>') # s)"
 
@@ -103,9 +95,6 @@ next
   thus ?case by (induction rule: eval\<^sub>e.cases) simp_all 
 next
   case ev\<^sub>e_pushenv
-  thus ?case by (induction rule: eval\<^sub>e.cases) simp_all 
-next
-  case ev\<^sub>e_popenv
   thus ?case by (induction rule: eval\<^sub>e.cases) simp_all 
 next
   case ev\<^sub>e_return
