08ByteCode/CodeFlattening.thy
@@ -19,22 +19,21 @@ fun flatten_code' :: "nat \<Rightarrow> code\<^sub>e list \<Rightarrow> code\<^s
     in \<C>\<^sub>b' @ flatten_code' (p + length \<C>\<^sub>b') \<C> @ [PushLam\<^sub>b (p + length \<C>\<^sub>b') n])"
 | "flatten_code' p (Apply\<^sub>e # \<C>) = flatten_code' p \<C> @ [Apply\<^sub>b]"
 | "flatten_code' p (PushEnv\<^sub>e # \<C>) = flatten_code' p \<C> @ [PushEnv\<^sub>b]"
-| "flatten_code' p (PopEnv\<^sub>e # \<C>) = undefined"
 | "flatten_code' p (Return\<^sub>e # \<C>) = flatten_code' p \<C> @ [Return\<^sub>b]"
 | "flatten_code' p (Jump\<^sub>e # \<C>) = flatten_code' p \<C> @ [Jump\<^sub>b]"
 
 definition flatten_code :: "code\<^sub>e list \<Rightarrow> code\<^sub>b list" where
   "flatten_code \<C> \<equiv> flatten_code' 0 \<C>"
 
-lemma properly_terminated_flatten' [simp]: "properly_terminated\<^sub>e \<C> \<Longrightarrow> pop_free \<C> \<Longrightarrow>
+lemma properly_terminated_flatten' [simp]: "properly_terminated\<^sub>e \<C> \<Longrightarrow> 
     properly_terminated\<^sub>b (flatten_code' p \<C> @ \<C>')"
   by (induction p \<C> arbitrary: \<C>' rule: flatten_code'.induct) 
      (auto simp add: Let_def split: if_splits)
 
-lemma properly_terminated_flatten [simp]: "properly_terminated\<^sub>e \<C> \<Longrightarrow> pop_free \<C> \<Longrightarrow>
+lemma properly_terminated_flatten [simp]: "properly_terminated\<^sub>e \<C> \<Longrightarrow> 
   properly_terminated\<^sub>b (flatten_code \<C>)"
 proof (unfold flatten_code_def)
-  assume "properly_terminated\<^sub>e \<C>" and "pop_free \<C>"
+  assume "properly_terminated\<^sub>e \<C>"
   hence "properly_terminated\<^sub>b (flatten_code' 0 \<C> @ [])" by (metis properly_terminated_flatten')
   thus "properly_terminated\<^sub>b (flatten_code' 0 \<C>)" by simp
 qed
@@ -50,23 +49,22 @@ primrec code_size :: "code\<^sub>e \<Rightarrow> nat"
 | "code_size (PushLam\<^sub>e \<C> n) = Suc (code_list_size \<C>)"
 | "code_size Apply\<^sub>e = 1"
 | "code_size PushEnv\<^sub>e = 1"
-| "code_size PopEnv\<^sub>e = undefined"
 | "code_size Return\<^sub>e = 1"
 | "code_size Jump\<^sub>e = 1"
 | "code_list_size [] = 0"
 | "code_list_size (op # \<C>) = code_size op + code_list_size \<C>"
 
-lemma length_flatten' [simp]: "pop_free \<C> \<Longrightarrow> length (flatten_code' p \<C>) = code_list_size \<C>"
+lemma length_flatten' [simp]: "length (flatten_code' p \<C>) = code_list_size \<C>"
   by (induction p \<C> rule: flatten_code'.induct) simp_all
 
-lemma length_flatten [simp]: "pop_free \<C> \<Longrightarrow> length (flatten_code \<C>) = code_list_size \<C>"
+lemma length_flatten [simp]: "length (flatten_code \<C>) = code_list_size \<C>"
   by (simp add: flatten_code_def)
 
-lemma code_size_nz [simp]: "op \<noteq> PopEnv\<^sub>e \<Longrightarrow> 0 < code_size op"
+lemma code_size_nz [simp]: "0 < code_size op"
   by (induction op) simp_all
 
-lemma code_list_size_empty [simp]: "pop_free \<C> \<Longrightarrow> (code_list_size \<C> = 0) = (\<C> = [])"
-  by (induction \<C> rule: pop_free.induct) simp_all
+lemma code_list_size_empty [simp]: "(code_list_size \<C> = 0) = (\<C> = [])"
+  by (induction \<C>) simp_all
 
 lemma index_into_append [simp]: "pop_free \<C> \<Longrightarrow> 
     lookup (flatten_code' m \<C> @ \<C>') (code_list_size \<C> + n) = lookup \<C>' n"
@@ -123,7 +121,7 @@ primrec unflatten_state :: "code\<^sub>b list \<Rightarrow> state\<^sub>b \<Righ
 lemma unflatten_front [simp]: "p \<le> length \<C> \<Longrightarrow> unflatten_code (\<C> @ \<C>') p = unflatten_code \<C> p"
   by (induction \<C> p rule: unflatten_code.induct) (simp_all split: option.splits code\<^sub>b.splits) 
 
-lemma unflatten_flatten' [simp]: "properly_terminated\<^sub>e \<C> \<Longrightarrow> pop_free \<C> \<Longrightarrow> 
+lemma unflatten_flatten' [simp]: "properly_terminated\<^sub>e \<C> \<Longrightarrow> 
   unflatten_code (\<C>' @ flatten_code' (length \<C>') \<C> @ \<C>'') (length \<C>' + code_list_size \<C>) = \<C>"
 proof (induction "length \<C>'" \<C> arbitrary: \<C>' \<C>'' rule: flatten_code'.induct)
   case (4 \<C>\<^sub>2 n \<C>\<^sub>1)
@@ -131,24 +129,24 @@ proof (induction "length \<C>'" \<C> arbitrary: \<C>' \<C>'' rule: flatten_code'
   let ?code' = "\<C>' @ flatten_code' (length \<C>') \<C>\<^sub>2 @ []"
   let ?code = "?code' @ flatten_code' ?pc \<C>\<^sub>1 @ PushLam\<^sub>b ?pc n # \<C>''"
   have X: "length \<C>' + length (flatten_code' (length \<C>') \<C>\<^sub>2) = length ?code'" by simp
-  from 4 have "properly_terminated\<^sub>e \<C>\<^sub>1 \<and> pop_free \<C>\<^sub>1" by simp
+  from 4 have "properly_terminated\<^sub>e \<C>\<^sub>1" by simp
   with 4 X have "unflatten_code (?code' @ flatten_code' (length ?code') \<C>\<^sub>1 @
     PushLam\<^sub>b (length \<C>' + length (flatten_code' (length \<C>') \<C>\<^sub>2)) n # \<C>'')
       (length ?code' + code_list_size \<C>\<^sub>1) = \<C>\<^sub>1" by blast
   with 4 have "unflatten_code ?code (length \<C>' + code_list_size \<C>\<^sub>2 + code_list_size \<C>\<^sub>1) = \<C>\<^sub>1" by simp
   hence X: "unflatten_code ?code (length \<C>' + (code_list_size \<C>\<^sub>2 + code_list_size \<C>\<^sub>1)) = \<C>\<^sub>1" 
     by (metis add.assoc)
-  from 4 have "properly_terminated\<^sub>e \<C>\<^sub>2 \<and> pop_free \<C>\<^sub>2" by simp
+  from 4 have "properly_terminated\<^sub>e \<C>\<^sub>2" by simp
   with 4 have "unflatten_code ?code' (length \<C>' + code_list_size \<C>\<^sub>2) = \<C>\<^sub>2" by blast
   moreover from 4 have "?pc \<le> length ?code'" by simp
   ultimately have Z: "unflatten_code ?code ?pc = \<C>\<^sub>2" by (metis unflatten_front)
   with 4 X Z show ?case by simp
 qed simp_all
 
-lemma unflatten_flatten [simp]: "properly_terminated\<^sub>e \<C> \<Longrightarrow> pop_free \<C> \<Longrightarrow> 
+lemma unflatten_flatten [simp]: "properly_terminated\<^sub>e \<C> \<Longrightarrow> 
   unflatten_code (flatten_code \<C>) (code_list_size \<C>) = \<C>"
 proof -
-  assume "properly_terminated\<^sub>e \<C>" and "pop_free \<C>"
+  assume "properly_terminated\<^sub>e \<C>"
   hence "unflatten_code ([] @ flatten_code' (length []) \<C> @ []) 
     (length [] + code_list_size \<C>) = \<C>" by (metis unflatten_flatten' list.size(3))
   thus ?thesis by (simp add: flatten_code_def)
@@ -183,25 +181,24 @@ lemma orderly_append [simp]: "orderly_code (\<C> @ \<C>') n =
     (orderly_code \<C> n \<and> orderly_code \<C>' (length \<C> + n))"
   by (induction \<C> arbitrary: n) simp_all
 
-lemma orderly_flatten' [simp]: "p \<le> n \<Longrightarrow> properly_terminated\<^sub>e \<C> \<Longrightarrow> pop_free \<C> \<Longrightarrow>
+lemma orderly_flatten' [simp]: "p \<le> n \<Longrightarrow> properly_terminated\<^sub>e \<C> \<Longrightarrow> 
     orderly_code (flatten_code' p \<C>) n"
   by (induction p \<C> arbitrary: n rule: flatten_code'.induct) auto
 
-lemma orderly_flatten [simp]: "properly_terminated\<^sub>e \<C> \<Longrightarrow> pop_free \<C> \<Longrightarrow> 
-    orderly_code (flatten_code \<C>) 0"
+lemma orderly_flatten [simp]: "properly_terminated\<^sub>e \<C> \<Longrightarrow> orderly_code (flatten_code \<C>) 0"
   by (simp add: flatten_code_def)
 
 lemma orderly_empty_frame [simp]: "x > 0 \<Longrightarrow> orderly_stack [([], x)] x"
   by (cases x) simp_all
 
-lemma orderly_length_flatten [simp]: "\<C> \<noteq> [] \<Longrightarrow> pop_free \<C> \<Longrightarrow>
+lemma orderly_length_flatten [simp]: "\<C> \<noteq> [] \<Longrightarrow> 
     orderly_stack [([], length (flatten_code \<C>))] (length (flatten_code \<C>))"
-  by (induction \<C> rule: pop_free.induct) simp_all
+  by (induction \<C>) simp_all
 
-lemma orderly_code_size [simp]: "\<C> \<noteq> [] \<Longrightarrow> pop_free \<C> \<Longrightarrow>
+lemma orderly_code_size [simp]: "\<C> \<noteq> [] \<Longrightarrow> 
     orderly_stack [([], code_list_size \<C>)] (code_list_size \<C>)"
 proof -
-  assume "\<C> \<noteq> []" and "pop_free \<C>"
+  assume "\<C> \<noteq> []"
   moreover hence "orderly_stack [([], length (flatten_code \<C>))] (length (flatten_code \<C>))" 
     by (metis orderly_length_flatten)
   ultimately show ?thesis by simp
@@ -348,10 +345,6 @@ lemma unflatten_to_pushenv [dest]: "PushEnv\<^sub>e # \<C>\<^sub>e = unflatten_c
      orderly_code \<C>\<^sub>b 0 \<Longrightarrow> p < length \<C>\<^sub>b \<Longrightarrow> lookup \<C>\<^sub>b p = Some PushEnv\<^sub>b \<and> \<C>\<^sub>e = unflatten_code \<C>\<^sub>b p"
   by (simp split: option.splits code\<^sub>b.splits)
 
-lemma unflatten_to_pop [dest]: "PopEnv\<^sub>e # \<C>\<^sub>e = unflatten_code \<C>\<^sub>b (Suc p) \<Longrightarrow> orderly_code \<C>\<^sub>b 0 \<Longrightarrow>  
-    p < length \<C>\<^sub>b \<Longrightarrow>False"
-  by (simp split: option.splits code\<^sub>b.splits)
-
 lemma unflatten_to_return [dest]: "Return\<^sub>e # \<C>\<^sub>e = unflatten_code \<C>\<^sub>b (Suc p) \<Longrightarrow> 
     orderly_code \<C>\<^sub>b 0 \<Longrightarrow> p < length \<C>\<^sub>b \<Longrightarrow> lookup \<C>\<^sub>b p = Some Return\<^sub>b \<and> \<C>\<^sub>e = []"
   by (simp split: option.splits code\<^sub>b.splits)
@@ -416,11 +409,6 @@ proof (induction s\<^sub>b "length \<C>\<^sub>b" rule: orderly_stack.induct)
   hence "lookup \<C>\<^sub>b p = Some PushEnv\<^sub>b \<and> \<C>\<^sub>e = unflatten_code \<C>\<^sub>b p" by blast
   with 3 show ?case by simp
 qed simp_all
-
-lemma unflatten_stack_to_pop [dest]: "(\<Delta>\<^sub>e, PopEnv\<^sub>e # \<C>\<^sub>e) # s\<^sub>e = unflatten_stack \<C>\<^sub>b s\<^sub>b \<Longrightarrow> 
-    orderly_code \<C>\<^sub>b 0 \<Longrightarrow> orderly_stack s\<^sub>b (length \<C>\<^sub>b) \<Longrightarrow> False"
-  by (induction s\<^sub>b "length \<C>\<^sub>b" rule: orderly_stack.induct) 
-     (simp_all split: option.splits code\<^sub>b.splits)
 
 lemma unflatten_stack_to_return [dest]: "(\<Delta>\<^sub>e, Return\<^sub>e # \<C>\<^sub>e) # s\<^sub>e = unflatten_stack \<C>\<^sub>b s\<^sub>b \<Longrightarrow> 
   orderly_code \<C>\<^sub>b 0 \<Longrightarrow> orderly_stack s\<^sub>b (length \<C>\<^sub>b) \<Longrightarrow> \<exists>\<Delta>\<^sub>b p s\<^sub>b'. s\<^sub>b = (\<Delta>\<^sub>b, Suc p) # s\<^sub>b' \<and> 
@@ -522,12 +510,6 @@ next
   hence "iter (\<tturnstile> \<C>\<^sub>b \<leadsto>\<^sub>b) (S\<^sub>b (v\<^sub>b # \<V>\<^sub>b') ((\<Delta>\<^sub>b, Suc p) # s\<^sub>b')) (S\<^sub>b \<V>\<^sub>b' ((cons_fst v\<^sub>b \<Delta>\<^sub>b, p) # s\<^sub>b'))" 
     by simp
   with B E V show ?case by auto
-next
-  case (ev\<^sub>e_popenv \<V> v vs \<Delta> \<C> s)
-  then obtain \<V>\<^sub>b s\<^sub>b where "\<Sigma>\<^sub>b = S\<^sub>b \<V>\<^sub>b s\<^sub>b \<and> \<V> = unflatten_values \<C>\<^sub>b \<V>\<^sub>b \<and> 
-    (((v # vs) # \<Delta>, PopEnv\<^sub>e # \<C>) # s) = unflatten_stack \<C>\<^sub>b s\<^sub>b" by fastforce
-  moreover with ev\<^sub>e_popenv have "orderly_code \<C>\<^sub>b 0 \<and> orderly_stack s\<^sub>b (length \<C>\<^sub>b)" by simp
-  ultimately show ?case by (metis unflatten_stack_to_pop)
 next
   case (ev\<^sub>e_return \<V>\<^sub>e \<Delta>\<^sub>e \<C>\<^sub>e s\<^sub>e)
   then obtain \<V>\<^sub>b s\<^sub>b where B: "\<Sigma>\<^sub>b = S\<^sub>b \<V>\<^sub>b s\<^sub>b \<and> \<V>\<^sub>e = unflatten_values \<C>\<^sub>b \<V>\<^sub>b \<and> 
